a checkpoint with axiomatized, renamed modules

examples/ghc/lib/CoAxiom.v
@@ -28,87 +28,19 @@ Require Unique.
 Definition TypeEqn :=
   (Pair.Pair AxiomatizedTypes.Type_)%type.
 
-Inductive CoAxiomRule : Type
-  := | Mk_CoAxiomRule (coaxrName : FastString.FastString) (coaxrAsmpRoles
-    : list AxiomatizedTypes.Role) (coaxrRole : AxiomatizedTypes.Role) (coaxrProves
-    : list TypeEqn -> option TypeEqn)
-   : CoAxiomRule.
-
-Inductive CoAxBranch : Type
-  := | Mk_CoAxBranch (cab_loc : SrcLoc.SrcSpan) (cab_tvs : list Core.TyVar)
-  (cab_cvs : list Core.CoVar) (cab_roles : list AxiomatizedTypes.Role) (cab_lhs
-    : list AxiomatizedTypes.Type_) (cab_rhs : AxiomatizedTypes.Type_) (cab_incomps
-    : list CoAxBranch)
-   : CoAxBranch.
-
 Axiom Branches : Type -> Type.
-
-Definition BranchIndex :=
-  nat%type.
 
 Inductive BranchFlag : Type
   := | Branched : BranchFlag
   |  Unbranched : BranchFlag.
 
-Instance Default__CoAxiomRule : GHC.Err.Default CoAxiomRule :=
-  GHC.Err.Build_Default _ (Mk_CoAxiomRule GHC.Err.default GHC.Err.default
-                         GHC.Err.default GHC.Err.default).
-
-Instance Default__CoAxBranch : GHC.Err.Default CoAxBranch :=
-  GHC.Err.Build_Default _ (Mk_CoAxBranch GHC.Err.default GHC.Err.default
-                         GHC.Err.default GHC.Err.default GHC.Err.default GHC.Err.default
-                         GHC.Err.default).
-
 Instance Default__BranchFlag : GHC.Err.Default BranchFlag :=
   GHC.Err.Build_Default _ Branched.
 
-Definition coaxrAsmpRoles (arg_0__ : CoAxiomRule) :=
-  let 'Mk_CoAxiomRule _ coaxrAsmpRoles _ _ := arg_0__ in
-  coaxrAsmpRoles.
-
-Definition coaxrName (arg_0__ : CoAxiomRule) :=
-  let 'Mk_CoAxiomRule coaxrName _ _ _ := arg_0__ in
-  coaxrName.
-
-Definition coaxrProves (arg_0__ : CoAxiomRule) :=
-  let 'Mk_CoAxiomRule _ _ _ coaxrProves := arg_0__ in
-  coaxrProves.
-
-Definition coaxrRole (arg_0__ : CoAxiomRule) :=
-  let 'Mk_CoAxiomRule _ _ coaxrRole _ := arg_0__ in
-  coaxrRole.
-
-Definition cab_cvs (arg_0__ : CoAxBranch) :=
-  let 'Mk_CoAxBranch _ _ cab_cvs _ _ _ _ := arg_0__ in
-  cab_cvs.
-
-Definition cab_incomps (arg_0__ : CoAxBranch) :=
-  let 'Mk_CoAxBranch _ _ _ _ _ _ cab_incomps := arg_0__ in
-  cab_incomps.
-
-Definition cab_lhs (arg_0__ : CoAxBranch) :=
-  let 'Mk_CoAxBranch _ _ _ _ cab_lhs _ _ := arg_0__ in
-  cab_lhs.
-
-Definition cab_loc (arg_0__ : CoAxBranch) :=
-  let 'Mk_CoAxBranch cab_loc _ _ _ _ _ _ := arg_0__ in
-  cab_loc.
-
-Definition cab_rhs (arg_0__ : CoAxBranch) :=
-  let 'Mk_CoAxBranch _ _ _ _ _ cab_rhs _ := arg_0__ in
-  cab_rhs.
-
-Definition cab_roles (arg_0__ : CoAxBranch) :=
-  let 'Mk_CoAxBranch _ _ _ cab_roles _ _ _ := arg_0__ in
-  cab_roles.
-
-Definition cab_tvs (arg_0__ : CoAxBranch) :=
-  let 'Mk_CoAxBranch _ cab_tvs _ _ _ _ _ := arg_0__ in
-  cab_tvs.
-
 (* Converted value declarations: *)
 
-Axiom unbranched : CoAxBranch -> Branches AxiomatizedTypes.Unbranched.
+Axiom unbranched : AxiomatizedTypes.CoAxBranch ->
+                   Branches AxiomatizedTypes.Unbranched.
 
 Axiom trivialBuiltInFamily : AxiomatizedTypes.BuiltInSynFamily.
 
@@ -126,29 +58,33 @@ Axiom toBranchedAxiom : forall {br},
 Axiom toBranched : forall {br},
                    Branches br -> Branches AxiomatizedTypes.Branched.
 
-Axiom placeHolderIncomps : list CoAxBranch.
+Axiom placeHolderIncomps : list AxiomatizedTypes.CoAxBranch.
 
 Axiom numBranches : forall {br}, Branches br -> nat.
 
 Axiom mapAccumBranches : forall {br},
-                         (list CoAxBranch -> CoAxBranch -> CoAxBranch) -> Branches br -> Branches br.
+                         (list AxiomatizedTypes.CoAxBranch ->
+                          AxiomatizedTypes.CoAxBranch -> AxiomatizedTypes.CoAxBranch) ->
+                         Branches br -> Branches br.
 
-Axiom manyBranches : list CoAxBranch -> Branches AxiomatizedTypes.Branched.
+Axiom manyBranches : list AxiomatizedTypes.CoAxBranch ->
+                     Branches AxiomatizedTypes.Branched.
 
 Axiom isImplicitCoAxiom : forall {br}, AxiomatizedTypes.CoAxiom br -> bool.
 
 Axiom fsFromRole : AxiomatizedTypes.Role -> FastString.FastString.
 
-Axiom fromBranches : forall {br}, Branches br -> list CoAxBranch.
+Axiom fromBranches : forall {br},
+                     Branches br -> list AxiomatizedTypes.CoAxBranch.
 
 Axiom coAxiomTyCon : forall {br}, AxiomatizedTypes.CoAxiom br -> Core.TyCon.
 
 Axiom coAxiomSingleBranch_maybe : forall {br},
-                                  AxiomatizedTypes.CoAxiom br -> option CoAxBranch.
+                                  AxiomatizedTypes.CoAxiom br -> option AxiomatizedTypes.CoAxBranch.
 
 Axiom coAxiomSingleBranch : AxiomatizedTypes.CoAxiom
                             AxiomatizedTypes.Unbranched ->
-                            CoAxBranch.
+                            AxiomatizedTypes.CoAxBranch.
 
 Axiom coAxiomRole : forall {br},
                     AxiomatizedTypes.CoAxiom br -> AxiomatizedTypes.Role.
@@ -156,30 +92,35 @@ Axiom coAxiomRole : forall {br},
 Axiom coAxiomNumPats : forall {br}, AxiomatizedTypes.CoAxiom br -> nat.
 
 Axiom coAxiomNthBranch : forall {br},
-                         AxiomatizedTypes.CoAxiom br -> BranchIndex -> CoAxBranch.
+                         AxiomatizedTypes.CoAxiom br ->
+                         AxiomatizedTypes.BranchIndex -> AxiomatizedTypes.CoAxBranch.
 
 Axiom coAxiomName : forall {br}, AxiomatizedTypes.CoAxiom br -> Name.Name.
 
 Axiom coAxiomBranches : forall {br}, AxiomatizedTypes.CoAxiom br -> Branches br.
 
 Axiom coAxiomArity : forall {br},
-                     AxiomatizedTypes.CoAxiom br -> BranchIndex -> BasicTypes.Arity.
+                     AxiomatizedTypes.CoAxiom br -> AxiomatizedTypes.BranchIndex -> BasicTypes.Arity.
 
-Axiom coAxBranchTyVars : CoAxBranch -> list Core.TyVar.
+Axiom coAxBranchTyVars : AxiomatizedTypes.CoAxBranch -> list Core.TyVar.
 
-Axiom coAxBranchSpan : CoAxBranch -> SrcLoc.SrcSpan.
+Axiom coAxBranchSpan : AxiomatizedTypes.CoAxBranch -> SrcLoc.SrcSpan.
 
-Axiom coAxBranchRoles : CoAxBranch -> list AxiomatizedTypes.Role.
+Axiom coAxBranchRoles : AxiomatizedTypes.CoAxBranch ->
+                        list AxiomatizedTypes.Role.
 
-Axiom coAxBranchRHS : CoAxBranch -> AxiomatizedTypes.Type_.
+Axiom coAxBranchRHS : AxiomatizedTypes.CoAxBranch -> AxiomatizedTypes.Type_.
 
-Axiom coAxBranchLHS : CoAxBranch -> list AxiomatizedTypes.Type_.
+Axiom coAxBranchLHS : AxiomatizedTypes.CoAxBranch ->
+                      list AxiomatizedTypes.Type_.
 
-Axiom coAxBranchIncomps : CoAxBranch -> list CoAxBranch.
+Axiom coAxBranchIncomps : AxiomatizedTypes.CoAxBranch ->
+                          list AxiomatizedTypes.CoAxBranch.
 
-Axiom coAxBranchCoVars : CoAxBranch -> list Core.CoVar.
+Axiom coAxBranchCoVars : AxiomatizedTypes.CoAxBranch -> list Core.CoVar.
 
-Axiom branchesNth : forall {br}, Branches br -> BranchIndex -> CoAxBranch.
+Axiom branchesNth : forall {br},
+                    Branches br -> AxiomatizedTypes.BranchIndex -> AxiomatizedTypes.CoAxBranch.
 
 Instance Eq___Role : GHC.Base.Eq_ AxiomatizedTypes.Role := {}.
 Proof.
@@ -231,15 +172,17 @@ Admitted.
 (* Skipping all instances of class `Outputable.Outputable', including
    `CoAxiom.Outputable__CoAxiomRule' *)
 
-Instance Eq___CoAxiomRule : GHC.Base.Eq_ CoAxiomRule := {}.
+Instance Ord__CoAxiomRule : GHC.Base.Ord AxiomatizedTypes.CoAxiomRule := {}.
 Proof.
 Admitted.
 
-Instance Ord__CoAxiomRule : GHC.Base.Ord CoAxiomRule := {}.
+Instance Eq___CoAxiomRule : GHC.Base.Eq_ AxiomatizedTypes.CoAxiomRule := {}.
 Proof.
 Admitted.
 
-Instance Uniquable__CoAxiomRule : Unique.Uniquable CoAxiomRule := {}.
+Instance Uniquable__CoAxiomRule
+   : Unique.Uniquable AxiomatizedTypes.CoAxiomRule :=
+  {}.
 Proof.
 Admitted.
 
@@ -247,10 +190,11 @@ Admitted.
    `CoAxiom.Data__CoAxiomRule' *)
 
 (* External variables:
-     Type bool list nat option AxiomatizedTypes.Branched
-     AxiomatizedTypes.BuiltInSynFamily AxiomatizedTypes.CoAxiom AxiomatizedTypes.Role
+     Type bool list nat option AxiomatizedTypes.BranchIndex AxiomatizedTypes.Branched
+     AxiomatizedTypes.BuiltInSynFamily AxiomatizedTypes.CoAxBranch
+     AxiomatizedTypes.CoAxiom AxiomatizedTypes.CoAxiomRule AxiomatizedTypes.Role
      AxiomatizedTypes.Type_ AxiomatizedTypes.Unbranched BasicTypes.Arity Core.CoVar
      Core.TyCon Core.TyVar FastString.FastString GHC.Base.Eq_ GHC.Base.Ord
-     GHC.Err.Build_Default GHC.Err.Default GHC.Err.default Name.Name Name.NamedThing
-     Pair.Pair SrcLoc.SrcSpan Unique.Uniquable
+     GHC.Err.Build_Default GHC.Err.Default Name.Name Name.NamedThing Pair.Pair
+     SrcLoc.SrcSpan Unique.Uniquable
 *)
